infoflow: weakened assumptions for c refinement of infoflow adts
The fact that the C infoflow adt refines the abstract infoflow adt now only requires that given user operation is nonempty and not sane (nonempty and doesn't return an interrupt).
Also added some more general lemmas about fw_sim and refinement to lib/Simulation.thy.

proof/infoflow/ADT_IF_Refine.thy
@@ -1031,11 +1031,7 @@ definition ADT_H_if where
                               kernelCall_H_if handlePreemption_H_if
                               schedule'_H_if kernelExit_H_if)\<rparr>"
 
-definition uop_sane  where
-"uop_sane f \<equiv> \<forall>t pl pr pxn tcu. (f t pl pr pxn tcu) \<noteq> {} \<and> 
-                (\<forall>tc um es. (Some Interrupt,tc,um, es) \<notin> (f t pl pr pxn tcu))"
-
-lemma haskell_invs: "uop_sane uop \<Longrightarrow> global_automaton_invs checkActiveIRQ_H_if (doUserOp_H_if uop)
+lemma haskell_invs: "global_automaton_invs checkActiveIRQ_H_if (doUserOp_H_if uop)
                                      kernelCall_H_if handlePreemption_H_if
                                      schedule'_H_if kernelExit_H_if full_invs_if' (ADT_H_if uop) UNIV"
   apply (unfold_locales)
@@ -1044,11 +1040,11 @@ lemma haskell_invs: "uop_sane uop \<Longrightarrow> global_automaton_invs checkA
   apply (simp_all add: checkActiveIRQ_H_if_def doUserOp_H_if_def 
                                     kernelCall_H_if_def handlePreemption_H_if_def
                                     schedule'_H_if_def kernelExit_H_if_def split del: split_if)[12]
-             apply (rule preserves_lifts | wp | simp add: full_invs_if'_def uop_sane_def)+
+             apply (rule preserves_lifts | wp | simp add: full_invs_if'_def)+
            apply (wp_once hoare_disjI1)
-            apply (rule preserves_lifts | wp | simp add: full_invs_if'_def uop_sane_def)+
+            apply (rule preserves_lifts | wp | simp add: full_invs_if'_def)+
           apply (wp_once hoare_disjI2)
-           apply (rule preserves_lifts | wp | simp add: full_invs_if'_def uop_sane_def)+
+           apply (rule preserves_lifts | wp | simp add: full_invs_if'_def)+
            apply (rule hoare_pre)
             apply (rule hoare_vcg_conj_lift)
              apply (rule hoare_drop_imps)
@@ -1171,13 +1167,16 @@ lemma extras_inter'[dest!]: "(t,mode) \<in> has_srel_state (lift_fst_rel srel) i
     apply (fastforce intro!: srel_Fin simp: lift_fst_rel_def)
     done
 
-  lemma refinement: "ADT_conc \<sqsubseteq> ADT_abs"
-    apply (rule sim_imp_refines)
+  lemma fw_simulates: "ADT_conc \<sqsubseteq>\<^sub>F ADT_abs"
     apply (rule L_invariantI)
       apply (rule abs.ADT_invs)
      apply (rule conc.ADT_invs)
     apply (rule fw_sim_abs_conc)
-   done
+    done
+
+  lemma refinement: "ADT_conc \<sqsubseteq> ADT_abs"
+    apply (rule sim_imp_refines[OF fw_simulates])
+    done
 
   lemma conc_serial:
     assumes uop_sane: "\<And>s e t. (s,e,t) \<in> do_user_op_conc \<Longrightarrow> 
@@ -1399,7 +1398,7 @@ lemma ct_idle'_related: "\<lbrakk>(a, c) \<in> state_relation; invs' c; ct_idle 
   apply (case_tac st, simp_all)[1]
   done
 
-lemma haskell_to_abs: "uop_sane uop \<Longrightarrow> global_automata_refine 
+lemma haskell_to_abs: "uop_nonempty uop \<Longrightarrow> global_automata_refine 
                                check_active_irq_A_if (do_user_op_A_if uop)
                                kernel_call_A_if kernel_handle_preemption_if
                                kernel_schedule_if kernel_exit_A_if 
@@ -1411,7 +1410,7 @@ lemma haskell_to_abs: "uop_sane uop \<Longrightarrow> global_automata_refine
   apply (simp add: global_automata_refine_def)
   apply (intro conjI)
     apply (rule abstract_invs)
-   apply (erule haskell_invs)
+   apply (rule haskell_invs)
   apply (unfold_locales)
            apply (simp add: step_restrict_def)
           apply (simp add: ADT_H_if_def ADT_A_if_def)
@@ -1443,8 +1442,8 @@ lemma haskell_to_abs: "uop_sane uop \<Longrightarrow> global_automata_refine
       apply (rule step_corres_lifts)
        apply (rule corres_guard_imp)
          apply (rule do_user_op_if_corres)
-        apply (fastforce simp: full_invs_if_def uop_sane_def)
-       apply (simp add: full_invs_if'_def uop_sane_def)
+        apply (fastforce simp: full_invs_if_def uop_nonempty_def)
+       apply (simp add: full_invs_if'_def uop_nonempty_def)
       apply (rule doUserOp_if_empty_fail)
      apply (simp add: kernelCall_H_if_def kernel_call_A_if_def)
      apply (rule step_corres_lifts)
@@ -1490,13 +1489,12 @@ lemma doUserOp_if_no_interrupt: "\<lbrace>K(uop_sane uop)\<rbrace> doUserOp_if u
   apply (clarsimp simp: uop_sane_def simp del: split_paired_All)
   done
 
-
 lemma ADT_A_if_Init_Fin_serial: "uop_sane uop \<Longrightarrow>
        Init_Fin_serial (ADT_A_if uop) s0 (full_invs_if \<inter> {s. step_restrict s})"
   apply (simp add: Init_Fin_serial_def)
   apply (rule conjI)
    apply (rule global_automata_refine.abs_serial[OF haskell_to_abs])
-      apply simp
+      apply (simp add: uop_sane_def uop_nonempty_def)
      apply (fastforce simp: step_restrict_def has_srel_state_def)
    apply (clarsimp simp add: doUserOp_H_if_def)
    apply (frule use_valid[OF _ doUserOp_if_no_interrupt])
@@ -1505,7 +1503,6 @@ lemma ADT_A_if_Init_Fin_serial: "uop_sane uop \<Longrightarrow>
    apply (clarsimp simp: ADT_A_if_def)+
   done
 
-
 lemma ADT_A_if_enabled:
   "uop_sane uop \<Longrightarrow> enabled_system (ADT_A_if uop) s0"
   apply (rule Init_Fin_serial.enabled)
@@ -1513,15 +1510,17 @@ lemma ADT_A_if_enabled:
   apply simp
   done
 
+lemma (in valid_initial_state_noenabled) uop_nonempty:
+  "uop_nonempty utf"
+  apply (simp add: uop_nonempty_def utf_non_empty)
+  done
+
 lemma (in valid_initial_state_noenabled) uop_sane:
   "uop_sane utf"
-  apply (simp add: uop_sane_def)
-   apply (intro allI conjI)
-    apply (cut_tac utf_non_empty)
-    apply blast
-   apply (cut_tac utf_non_interrupt)
-   apply blast
-   done
+  apply (simp add: uop_sane_def utf_non_empty)
+  apply (cut_tac utf_non_interrupt)
+  apply blast
+  done
 
 sublocale valid_initial_state_noenabled \<subseteq> valid_initial_state
   apply (unfold_locales)
